\documentclass{beamer}
\usetheme{purelyagile}

\usepackage[utf8]{inputenc}
\usepackage[T1]{fontenc}
\usepackage{helvet}
\usepackage{minted}

\title{Haskell programs: how do they run?}
\subtitle{Demystifying lazy evaluation}
\author{Tom Ellis}
\date{6th October 2016}

\begin{document}

\begin{frame}[t]
\titlepage
\end{frame}

\begin{frame}
\frametitle{A nice frame}
\framesubtitle{Subtitle}

\begin{itemize}
\item graph reduction
\item redex
\item weak head normal form (WHNF)
\item constant applicative form (CAF)
\item ``delays the evaluation of an expression until its value is needed''
\item call by need
\end{itemize}

I hope you will be able to work out everything else from first
principles.  Not everything is literally correct but it will give you
the right understanding for everything except the lowest level
performance hacking.

\end{frame}

\begin{frame}
  \frametitle{Normal form}

  \begin{itemize}
  \item literals
  \item variables
  \item constructors
  \item let
  \item lambda
  \item function application
  \item case
  \end{itemize}

  In a function application, the function itself and the arguments
  must be variables or literals.

  Constructors must be ``saturated'', i.e.\ no missing arguments.
\end{frame}

\begin{frame}[fragile]
  \frametitle{Normal form}
  \framesubtitle{Example}

  \begin{minted}{haskell}
    -- Haskell
    let x = 1 + 1
    f y = plus y (3 * y)
      where plus = (+)
    in f x

    -- Normal form
    let x = 1 + 1
        f = \y -> let plus = (+)
                      a1 = 3 * y
                  in plus y a1
    in f x
  \end{minted}

\end{frame}

\begin{frame}
\frametitle{Evaluation}
\framesubtitle{What do we evaluate to?}

The result of an evaluation is a ``value''.  A value is

\begin{itemize}
\item a (fully saturated) constructor (including primitive types), or
\item a lambda
\end{itemize}

\end{frame}

\begin{frame}[fragile]
  \frametitle{Evaluation}
  \framesubtitle{How do we evaluate?}

  \begin{itemize}
  \item literals -- already evaluated

  \item \verb+let x = e in body+: create a closure for \verb+e+ on the
    heap and let \verb+x+ be a pointer to this closure, i.e.\ all
    mentions of \verb+x+ scoped by this binding point to that closure.

  \item variables \verb+x+: \verb+x+ is a pointer to a closure.
    Evaluate that closure to a value and overwrite its memory location
    with the value (``memoization'').
  \item constructors -- already evaluated
  \item lambda -- already evaluated
  \item \verb+f a+: evaluate \verb+f+ to \verb+\x -> e+
  \item \verb+case e of alts+: evaluate \verb+e+, check which
    alternative matches and evaluate it
  \end{itemize}

\end{frame}

\begin{frame}[fragile]
  \frametitle{Evaluation}
  \framesubtitle{Heap and stack}

  \begin{itemize}
  \item The only thing that allocates on the heap is \verb+let+.

  \item The only thing that consumes stack (that we care about) is
    \verb+case+ whilst it is evaluating its scrutinee.
  \end{itemize}

\end{frame}

\iffalse

\begin{frame}[fragile]
\frametitle{Evaluation}
\framesubtitle{Evaluation example}

\begin{minted}{haskell}
    -- Evaluating
    let x = 1 + 1
        f = \y -> let plus = (+)
                      a1 = 3 * y
                  in plus y a1
    in f x
\end{minted}

\end{frame}

\begin{frame}[fragile]
\frametitle{Evaluation}
\framesubtitle{Evaluation example}

\begin{minted}{haskell}
    -- Evaluating
    f x

    -- Heap
    x = 1 + 1
    f = \y -> let plus = (+)
                  a1 = 3 * y
              in plus y a1
\end{minted}
\end{frame}

\begin{frame}[fragile]
\frametitle{Evaluation}
\framesubtitle{Evaluation example}

\begin{minted}{haskell}
    -- Evaluating
    let plus = (+)
        a1 = 3 * x
    in plus x a1

    -- Heap
    x = 1 + 1
    f = \y -> let plus = (+)
                  a1 = 3 * y
              in plus y a1
\end{minted}
\end{frame}

\begin{frame}[fragile]
\frametitle{Evaluation}
\framesubtitle{Evaluation example}

\begin{minted}{haskell}
    -- Evaluating
    plus x a1

    -- Heap
    x = 1 + 1
    f = \y -> let plus = (+)
                  a1 = 3 * y
              in plus y a1
    plus = (+)
    a1 = 3 * x
\end{minted}
\end{frame}

\begin{frame}[fragile]
\frametitle{Evaluation}
\framesubtitle{Evaluation example}

\begin{minted}{haskell}
    -- Evaluating
    (+) x a1

    -- Heap
    x = 1 + 1
    f = \y -> let plus = (+)
                  a1 = 3 * y
              in plus y a1
    plus = (+)
    a1 = 3 * x
\end{minted}
\end{frame}

\begin{frame}[fragile]
\frametitle{Evaluation}
\framesubtitle{Evaluation example}

\begin{minted}{haskell}
    -- Evaluating
    (+) x a1 | a1

    -- Heap
    x = 1 + 1
    f = \y -> let plus = (+)
                  a1 = 3 * y
              in plus y a1
    plus = (+)
    a1 = 3 * x
\end{minted}
\end{frame}

\begin{frame}[fragile]
\frametitle{Evaluation}
\framesubtitle{Evaluation example}

\begin{minted}{haskell}
    -- Evaluating
    (+) x a1 | a1 = 3 * x

    -- Heap
    x = 1 + 1
    f = \y -> let plus = (+)
                  a1 = 3 * y
              in plus y a1
    plus = (+)
    a1 = 3 * x
\end{minted}
\end{frame}

\begin{frame}[fragile]
\frametitle{Evaluation}
\framesubtitle{Evaluation example}

\begin{minted}{haskell}
    -- Evaluating
    (+) x a1 | a1 = 3 * x | x

    -- Heap
    x = 1 + 1
    f = \y -> let plus = (+)
                  a1 = 3 * y
              in plus y a1
    plus = (+)
    a1 = 3 * x
\end{minted}
\end{frame}

\begin{frame}[fragile]
\frametitle{Evaluation}
\framesubtitle{Evaluation example}

\begin{minted}{haskell}
    -- Evaluating
    (+) x a1 | a1 = 3 * x | x = 1 + 1

    -- Heap
    x = 1 + 1
    f = \y -> let plus = (+)
                  a1 = 3 * y
              in plus y a1
    plus = (+)
    a1 = 3 * x
\end{minted}
\end{frame}

\begin{frame}[fragile]
\frametitle{Evaluation}
\framesubtitle{Evaluation example}

\begin{minted}{haskell}
    -- Evaluating
    (+) x a1 | a1 = 3 * x | x = 2

    -- Heap
    x = 2
    f = \y -> let plus = (+)
                  a1 = 3 * y
              in plus y a1
    plus = (+)
    a1 = 3 * x
\end{minted}
\end{frame}

\begin{frame}[fragile]
\frametitle{Evaluation}
\framesubtitle{Evaluation example}

\begin{minted}{haskell}
    -- Evaluating
    (+) x a1 | a1 = 3 * 2

    -- Heap
    x = 2
    f = \y -> let plus = (+)
                  a1 = 3 * y
              in plus y a1
    plus = (+)
    a1 = 3 * x
\end{minted}
\end{frame}

\begin{frame}[fragile]
\frametitle{Evaluation}
\framesubtitle{Evaluation example}

\begin{minted}{haskell}
    -- Evaluating
    (+) x a1 | a1 = 6

    -- Heap
    x = 2
    f = \y -> let plus = (+)
                  a1 = 3 * y
              in plus y a1
    plus = (+)
    a1 = 6
\end{minted}
\end{frame}

\begin{frame}[fragile]
\frametitle{Evaluation}
\framesubtitle{Evaluation example}

\begin{minted}{haskell}
    -- Evaluating
    (+) 2 6

    -- Heap
    x = 2
    f = \y -> let plus = (+)
                  a1 = 3 * y
              in plus y a1
    plus = (+)
    a1 = 6
\end{minted}
\end{frame}

\begin{frame}[fragile]
\frametitle{Evaluation}
\framesubtitle{Evaluation example}

\begin{minted}{haskell}
    -- Evaluating
    8 -- A value.  The end!

    -- Heap
    x = 2
    f = \y -> let plus = (+)
                  a1 = 3 * y
              in plus y a1
    plus = (+)
    a1 = 6
\end{minted}
\end{frame}

\begin{frame}[fragile]
\frametitle{Evaluation}
\framesubtitle{Evaluation example}

\begin{minted}{haskell}
fibs = 0 : 1 : zipWith (+) fibs (tail fibs)

zipWith f (x:xs) (y:ys) = f x y : zipWith f xs ys
zipWith _ _      _      = []

tail (x:xs) = xs

head (x:xs) = x
\end{minted}
\end{frame}

\begin{frame}[fragile]
\frametitle{Evaluation}
\framesubtitle{Evaluation example}

\begin{minted}{haskell}
fibs = 0 : 1 : zipWith (+) fibs (tail fibs)

fibs = let tailfibs = tail fibs
           fibs2    = zipWith (+) fibs tailfibs
           fibs1    = 1 : fibs2
       in fibs = 0 : fibs1
\end{minted}
\end{frame}

\begin{frame}[fragile]
\frametitle{Evaluation}
\framesubtitle{Evaluation example}

\begin{minted}{haskell}
zipWith f (x:xs) (y:ys) = f x y : zipWith f xs ys
zipWith _ _      _      = []

zipWith = \f xs ys -> case xs of
    []    -> []
    x:xs' -> case ys of
        []    -> []
        y:ys' -> let first = f x y
                     rest  = zipWith f xs' ys'   
                 in first : rest
\end{minted}
\end{frame}


\begin{frame}[fragile]
\frametitle{Evaluation}
\framesubtitle{Evaluation example}

\begin{minted}{haskell}
tail (x:xs) = xs

head (x:xs) = x

tail = \xs -> case xs of x:xs' -> xs

head = \xs -> case xs of x:xs' -> x
\end{minted}
\end{frame}


\begin{frame}[t,fragile]
\frametitle{Evaluation}
\framesubtitle{Evaluation example}
\begin{minted}{haskell}
let fibs      = ...
    zipWith   = ...
    head      = ...
    tail      = ...
    tailfibs1 = tail fibs
    tailfibs2 = tail tailfibs1
    tailfibs3 = tail tailfibs2
in head tailfibs3
\end{minted}
\end{frame}

\begin{frame}[t,fragile]
\frametitle{Evaluation}
\framesubtitle{Evaluation example}
\begin{minted}{haskell}
-- Evaluating
head tailfibs3

-- Heap
fibs      = ...
zipWith   = ...
head      = ...
tail      = \xs -> case xs of x:xs' -> xs'
tailfibs1 = tail fibs
tailfibs2 = tail tailfibs1
tailfibs3 = tail tailfibs2
\end{minted}
\end{frame}

\begin{frame}[t,fragile]
\frametitle{Evaluation}
\framesubtitle{Evaluation example}
\begin{minted}{haskell}
-- Evaluating
case tailfibs3 of x:xs' -> xs'

-- Heap
fibs      = ...
zipWith   = ...
head      = ...
tail      = \xs -> case xs of x:xs' -> xs'
tailfibs1 = tail fibs
tailfibs2 = tail tailfibs1
tailfibs3 = tail tailfibs2
\end{minted}
\end{frame}

\begin{frame}[t,fragile]
\frametitle{Evaluation}
\framesubtitle{Evaluation example}
\begin{minted}{haskell}
-- Evaluating
case tailfibs3 of x:xs' -> xs'
|
tailfibs3

-- Heap
fibs      = ...
zipWith   = ...
head      = ...
tail      = \xs -> case xs of x:xs' -> xs'
tailfibs1 = tail fibs
tailfibs2 = tail tailfibs1
tailfibs3 = tail tailfibs2
\end{minted}
\end{frame}

\begin{frame}[t,fragile]
\frametitle{Evaluation}
\framesubtitle{Evaluation example}
\begin{minted}{haskell}
-- Evaluating
case tailfibs3 of x:xs' -> xs
|
tailfibs3 = tail tailfibs2

-- Heap
fibs      = ...
zipWith   = ...
head      = ...
tail      = \xs -> case xs of x:xs' -> xs'
tailfibs1 = tail fibs
tailfibs2 = tail tailfibs1
tailfibs3 = tail tailfibs2
\end{minted}
\end{frame}

\begin{frame}[t,fragile]
\frametitle{Evaluation}
\framesubtitle{Evaluation example}
\begin{minted}{haskell}
-- Evaluating
case tailfibs3 of x:xs' -> xs'
|
tailfibs3 = case tailfibs2 of x:xs' -> xs' 

-- Heap
fibs      = ...
zipWith   = ...
head      = ...
tail      = \xs -> case xs of x:xs' -> xs'
tailfibs1 = tail fibs
tailfibs2 = tail tailfibs1
tailfibs3 = tail tailfibs2
\end{minted}
\end{frame}

\begin{frame}[t,fragile]
\frametitle{Evaluation}
\framesubtitle{Evaluation example}
\begin{minted}{haskell}
-- Evaluating
case tailfibs3 of x:xs' -> xs'
|
tailfibs3 = case tailfibs2 of x:xs' -> xs' 
|
tailfibs2

-- Heap
...
\end{minted}
\end{frame}

\begin{frame}[t,fragile]
\frametitle{Evaluation}
\framesubtitle{Evaluation example}
\begin{minted}{haskell}
-- Evaluating
case tailfibs3 of x:xs' -> xs'
|
tailfibs3 = case tailfibs2 of x:xs' -> xs' 
|
tailfibs2 = case tailfibs1 of x:xs' -> xs' 
|
tailfibs1 = case fibs of x:xs' -> xs'

-- Heap
...
\end{minted}
\end{frame}

\begin{frame}[t,fragile]
\frametitle{Evaluation}
\framesubtitle{Evaluation example}
\begin{minted}{haskell}
-- Evaluating
case tailfibs3 of x:xs' -> xs'
|
tailfibs3 = case tailfibs2 of x:xs' -> xs' 
|
tailfibs2 = case tailfibs1 of x:xs' -> xs' 
|
tailfibs1 = case fibs of x:xs' -> xs'
|
fibs

-- Heap
fibs = 0 : fibs1
...
\end{minted}
\end{frame}

\begin{frame}[t,fragile]
\frametitle{Evaluation}
\framesubtitle{Evaluation example}
\begin{minted}{haskell}
-- Evaluating
case tailfibs3 of x:xs' -> xs'
|
tailfibs3 = case tailfibs2 of x:xs' -> xs' 
|
tailfibs2 = case tailfibs1 of x:xs' -> xs' 
|
tailfibs1 = case fibs of x:xs' -> xs'
|
fibs = 0 : fibs1

-- Heap
fibs = 0 : fibs1
...
\end{minted}
\end{frame}

\begin{frame}[t,fragile]
\frametitle{Evaluation}
\framesubtitle{Evaluation example}
\begin{minted}{haskell}
-- Evaluating
case tailfibs3 of x:xs' -> xs'
|
tailfibs3 = case tailfibs2 of x:xs' -> xs' 
|
tailfibs2 = case tailfibs1 of x:xs' -> xs' 
|
tailfibs1 = fibs1

-- Heap
fibs = 0 : fibs1
...
\end{minted}
\end{frame}

\begin{frame}[t,fragile]
\frametitle{Evaluation}
\framesubtitle{Evaluation example}
\begin{minted}{haskell}
-- Evaluating
case tailfibs3 of x:xs' -> xs'
|
tailfibs3 = case tailfibs2 of x:xs' -> xs' 
|
tailfibs2 = case tailfibs1 of x:xs' -> xs' 
|
tailfibs1 = fibs1
|
fibs1 

-- Heap
fibs1 = 1 : fibs2
...
\end{minted}
\end{frame}

\begin{frame}[t,fragile]
\frametitle{Evaluation}
\framesubtitle{Evaluation example}
\begin{minted}{haskell}
-- Evaluating
case tailfibs3 of x:xs' -> xs'
|
tailfibs3 = case tailfibs2 of x:xs' -> xs' 
|
tailfibs2 = case tailfibs1 of x:xs' -> xs' 
|
tailfibs1 = 1 : fibs2

-- Heap
fibs1 = 
...
\end{minted}
\end{frame}

\begin{frame}[t,fragile]
\frametitle{Evaluation}
\framesubtitle{Evaluation example}
\begin{minted}{haskell}
-- Evaluating
case tailfibs3 of x:xs' -> xs'
|
tailfibs3 = case tailfibs2 of x:xs' -> xs' 
|
tailfibs2 = case 1 : fibs2 of x:xs' -> xs' 

-- Heap
...
\end{minted}
\end{frame}

\begin{frame}[t,fragile]
\frametitle{Evaluation}
\framesubtitle{Evaluation example}
\begin{minted}{haskell}
-- Evaluating
case tailfibs3 of x:xs' -> xs'
|
tailfibs3 = case tailfibs2 of x:xs' -> xs' 
|
tailfibs2 = fibs2
|
fibs2

-- Heap
fibs2 = zipWith (+) fibs tailfibs
\end{minted}
\end{frame}

\begin{frame}[t,fragile]
\frametitle{Evaluation}
\framesubtitle{Evaluation example}
\begin{minted}{haskell}
-- Evaluating
case tailfibs3 of x:xs' -> xs'
|
tailfibs3 = case tailfibs2 of x:xs' -> xs' 
|
tailfibs2 = fibs2
|
fibs2 = zipWith (+) fibs tailfibs

-- Heap
...
\end{minted}
\end{frame}
\fi

\begin{frame}[t,fragile]
\frametitle{Evaluation}
\framesubtitle{Evaluation example}
\begin{minted}{haskell}
repeat x = xs where xs = x : xs

repeat = \x -> let xs = x : xs
               in xs

head (x:xs) = x

head = \xs -> case xs of x:xs' -> x  
\end{minted}
\end{frame}

\begin{frame}[t,fragile]
\frametitle{Evaluation}
\framesubtitle{Evaluation example}
\begin{minted}{haskell}
map f []     = []
map f (x:xs) = f x : map f xs

map = \f xs -> case xs of
  []    -> []   
  x:xs' -> let first = f x
               rest  = map f xs'
           in first : rest
\end{minted}
\end{frame}

\begin{frame}[t,fragile]
\frametitle{Evaluation}
\framesubtitle{Evaluation example}
\begin{minted}{haskell}
head (map (\x -> x + x) (repeat (10 + 1)))

let f = \x -> x + x
    t = 10 + 1
    r = repeat t
    m = map f r
in head m
\end{minted}
\end{frame}

\begin{frame}[t,fragile]
\frametitle{Evaluation}
\framesubtitle{Evaluation example}
\begin{minted}{haskell}
-- Evaluating
let f = \x -> x + x
    t = 10 + 1
    r = repeat t
    m = map f r
in head m

-- Heap
map = ...
repeat = ...
head = ...
\end{minted}
\end{frame}

\begin{frame}[t,fragile]
\frametitle{Evaluation}
\framesubtitle{Evaluation example}
\begin{minted}{haskell}
-- Evaluating
head m

-- Heap
map = ...
repeat = ...
head = \xs -> case xs of x:xs' -> x
f = \x -> x + x
t = 10 + 1
r = repeat t
m = map f r
\end{minted}
\end{frame}

\begin{frame}[t,fragile]
\frametitle{Evaluation}
\framesubtitle{Evaluation example}
\begin{minted}{haskell}
-- Evaluating
case m of x:xs -> x

-- Heap
map = ...
repeat = ...
head = ...
f = \x -> x + x
t = 10 + 1
r = repeat t
m = map f r
\end{minted}
\end{frame}

\begin{frame}[t,fragile]
\frametitle{Evaluation}
\framesubtitle{Evaluation example}
\begin{minted}{haskell}
-- Evaluating
case m of x:xs -> x
|
m

-- Heap
map = ...
repeat = ...
head = ...
f = \x -> x + x
t = 10 + 1
r = repeat t
m = map f r
\end{minted}
\end{frame}

\begin{frame}[t,fragile]
\frametitle{Evaluation}
\framesubtitle{Evaluation example}
\begin{minted}{haskell}
-- Evaluating
case m of x:xs -> x
|
m = map f r

-- Heap
map = ...
repeat = ...
head = ...
f = \x -> x + x
t = 10 + 1
r = repeat t
m = map f r
\end{minted}
\end{frame}

\begin{frame}[t,fragile]
\frametitle{Evaluation}
\framesubtitle{Evaluation example}
\begin{minted}{haskell}
-- Evaluating
case m of x:xs -> x
|
m = case r of
  []    -> []   
  x:xs' -> let first = f x
               rest  = map f xs'
           in first : rest

-- Heap
r = repeat t
...
\end{minted}
\end{frame}

\begin{frame}[t,fragile]
\frametitle{Evaluation}
\framesubtitle{Evaluation example}
\begin{minted}{haskell}
-- Evaluating
case m of x:xs -> x
|
m = case r of
  []    -> []   
  x:xs' -> let first = f x
               rest  = map f xs'
           in first : rest
|
r

-- Heap
r = repeat t
...
\end{minted}
\end{frame}

\begin{frame}[t,fragile]
\frametitle{Evaluation}
\framesubtitle{Evaluation example}
\begin{minted}{haskell}
-- Evaluating
case m of x:xs -> x
|
m = case r of
  []    -> []   
  x:xs' -> let first = f x
               rest  = map f xs'
           in first : rest
|
r = repeat t

-- Heap
r = repeat t
...
\end{minted}
\end{frame}

\begin{frame}[t,fragile]
\frametitle{Evaluation}
\framesubtitle{Evaluation example}
\begin{minted}{haskell}
-- Evaluating
case m of x:xs -> x
|
m = case r of
  []    -> []   
  x:xs' -> let first = f x
               rest  = map f xs'
           in first : rest
|
r = let xs = t : xs
    in xs

-- Heap
r = repeat t
...
\end{minted}
\end{frame}

\begin{frame}[t,fragile]
\frametitle{Evaluation}
\framesubtitle{Evaluation example}
\begin{minted}{haskell}
-- Evaluating
case m of x:xs -> x
|
m = case r of
  []    -> []   
  x:xs' -> let first = f x
               rest  = map f xs'
           in first : rest
|
r = xs

-- Heap
xs = t : xs
r = repeat t
...
\end{minted}
\end{frame}

\begin{frame}[t,fragile]
\frametitle{Evaluation}
\framesubtitle{Evaluation example}
\begin{minted}{haskell}
-- Evaluating
case m of x:xs -> x
|
m = case r of
  []    -> []   
  x:xs' -> let first = f x
               rest  = map f xs'
           in first : rest
|
r = xs

-- Heap
xs = t : xs
r ---^
...
\end{minted}
\end{frame}

\begin{frame}[t,fragile]
\frametitle{Evaluation}
\framesubtitle{Evaluation example}
\begin{minted}{haskell}
-- Evaluating
case m of x:xs -> x
|
m = let first = f t
        rest  = map f xs
    in first : rest

-- Heap
xs = t : xs
r ---^
...
\end{minted}
\end{frame}

\begin{frame}[t,fragile]
\frametitle{Evaluation}
\framesubtitle{Evaluation example}
\begin{minted}{haskell}
-- Evaluating
case m of x:xs -> x
|
m = first : rest

-- Heap
xs = t : xs
r ---^
first = f t
rest  = map f xs
m = first : rest
...
\end{minted}
\end{frame}

\begin{frame}[t,fragile]
\frametitle{Evaluation}
\framesubtitle{Evaluation example}
\begin{minted}{haskell}
-- Evaluating
first

-- Heap
xs = t : xs
r ---^
first = f t
rest  = map f xs
...
\end{minted}
\end{frame}

\begin{frame}[t,fragile]
\frametitle{Evaluation}
\framesubtitle{Evaluation example}
\begin{minted}{haskell}
-- Evaluating
first = f t

-- Heap
xs = t : xs
r ---^
first = f t
rest  = map f xs
...
\end{minted}
\end{frame}

\begin{frame}[t,fragile]
\frametitle{Evaluation}
\framesubtitle{Evaluation example}
\begin{minted}{haskell}
-- Evaluating
first = t + t

-- Heap
xs = t : xs
r ---^
first = f t
rest  = map f xs
t = 10 + 1
...
\end{minted}
\end{frame}

\begin{frame}[t,fragile]
\frametitle{Evaluation}
\framesubtitle{Evaluation example}
\begin{minted}{haskell}
-- Evaluating
first = t + t
|
t = 10 + 1

-- Heap
xs = t : xs
r ---^
first = f t
rest  = map f xs
t = 10 + 1
...
\end{minted}
\end{frame}

\begin{frame}[t,fragile]
\frametitle{Evaluation}
\framesubtitle{Evaluation example}
\begin{minted}{haskell}
-- Evaluating
first = t + t
|
t = 11

-- Heap
xs = t : xs
r ---^
first = f t
rest  = map f xs
t = 11
...
\end{minted}
\end{frame}

\begin{frame}[t,fragile]
\frametitle{Evaluation}
\framesubtitle{Evaluation example}
\begin{minted}{haskell}
-- Evaluating
first = 11 + 11

-- Heap
xs = t : xs
r ---^
first = f t
rest  = map f xs
t = 11
...
\end{minted}
\end{frame}

\begin{frame}[t,fragile]
\frametitle{Evaluation}
\framesubtitle{Evaluation example}
\begin{minted}{haskell}
-- Evaluating
first = 22

-- Heap
xs = t : xs
r ---^
first = 22
rest  = map f xs
t = 11
...
\end{minted}
\end{frame}

\begin{frame}[t,fragile]
\frametitle{Evaluation}
\framesubtitle{Evaluation example}
\begin{minted}{haskell}
-- Finished evaluating!
22

-- Heap
xs = t : xs
r ---^
first = 22
rest  = map f xs
t = 11
...
\end{minted}
\end{frame}

\end{document}
